impl interpreter for binops, add value and stack datatypes

inversion_lemmas.v
@@ -1,12 +1,16 @@
 From mathcomp Require Import ssreflect.
-From Coq Require Import Program.Equality NArith ZArith_base List Extraction.
+From Coq Require Import Program.Equality NArith ZArith_base List Extraction Floats.
 Import ListNotations.
 
 Notation " P ** Q " := (prod P Q) (at level 95, right associativity).
 
+Inductive value : Set :=
+  | val_i32: nat -> value
+  | val_f32: float -> value
+.
+
 Inductive term : Set :=
-  | term_i32
-  | term_f32
+  | term_const: value -> term
   | term_addi32
   | term_SEQ: term -> term -> term
 .
@@ -20,9 +24,14 @@ Inductive function_type : Type :=
   | Tf (t1s : list value_type) (t2s : list value_type)
 .
 
+Inductive value_typing : value -> value_type -> Prop :=
+  | val_typing_i32: forall n, value_typing (val_i32 n) t_i32
+  | val_typing_f32: forall n, value_typing (val_f32 n) t_f32
+.
+
 Inductive typing : term -> function_type -> Prop :=
-  | typing_term_i32 : typing term_i32 (Tf [] [t_i32])
-  | typing_term_f32 : typing term_f32 (Tf [] [t_f32])
+  | typing_term_const : forall v vt,
+      value_typing v vt -> typing (term_const v) (Tf [] [vt])
   | typing_term_addi32 : typing term_addi32 (Tf [t_i32; t_i32] [t_i32])
   | typing_weaken : forall t t1s t2s ts,
       typing t (Tf t1s t2s) -> typing t (Tf (ts ++ t1s) (ts ++ t2s))
@@ -32,6 +41,7 @@ Inductive typing : term -> function_type -> Prop :=
       typing (term_SEQ t1 t2) (Tf t1s t2s)
 .
 
+(* Equality decidability lemmas *)
 Lemma value_type_eq_dec : forall t1 t2 : value_type,
   {t1 = t2} + {t1 <> t2}.
 Proof. decide equality. Qed.
@@ -40,44 +50,49 @@ Lemma value_type_list_eq_dec : forall l1 l2 : list value_type,
   {l1 = l2} + {l1 <> l2}.
 Proof. apply List.list_eq_dec. apply value_type_eq_dec. Qed.
 
+Lemma value_typing_deterministic : forall v vt1 vt2,
+  value_typing v vt1 -> value_typing v vt2 -> vt1 = vt2.
+Proof.
+  intros ??? Hvt1 Hvt2.
+  inversion Hvt1; inversion Hvt2; subst; try reflexivity; discriminate.
+Qed.
+
 (* Typing inversion lemmas *)
-Lemma term_i32_typing_inv : forall t t1s t2s,
-  t = term_i32 ->
-  typing t (Tf t1s t2s) ->
-  {ts & t1s = ts ** t2s = ts ++ [t_i32]}.
+(* XXX how to do this as sigma type? *)
+Lemma value_typing_inversion_i32 : forall v,
+  value_typing v t_i32 -> {n & v = val_i32 n}.
 Proof.
-  intros t t1s t2s Hterm Htype.
+  intros v Hvtype.
+  destruct v as [n|].
+  - exists n. reflexivity.
+  - Fail induction Hvtype.
+Admitted. (* TODO *)
+
+Lemma term_const_typing_inv : forall t v vt t1s t2s,
+  t = (term_const v) ->
+  value_typing v vt ->
+  typing t (Tf t1s t2s) ->
+  {ts & t1s = ts /\ t2s = ts ++ [vt]}.
+Proof.
+  intros t v vt t1s t2s Hterm Hvtype Htype.
   subst t.
   exists t1s; split => //.
-  dependent induction Htype; subst => //.
-  rewrite <- app_assoc; f_equal.
-  by apply IHHtype.
+  dependent induction Htype.
+  - assert (Heqvt : vt0 = vt).
+    { by apply (value_typing_deterministic v _ _ H Hvtype). }
+    rewrite Heqvt. reflexivity.
+  - rewrite <- app_assoc; f_equal.
+    by apply (IHHtype _ _ _ Hvtype); reflexivity.
 Qed.
 
-Lemma term_f32_typing_inv : forall t t1s t2s,
-  t = term_f32 ->
-  typing t (Tf t1s t2s) ->
-  {ts & t1s = ts ** t2s = ts ++ [t_f32]}.
-Proof.
-  intros t t1s t2s Hterm Htype.
-  subst t.
-  exists t1s; split => //.
-  dependent induction Htype; subst => //.
-  rewrite <- app_assoc; f_equal.
-  by apply IHHtype.
-Qed.
-
-(* XXX do these need sigma types or is exists fine?
- * since we don't want to have them at runtime anyway *)
 (* TODO might need to use the type checker for this one too? *)
 Lemma term_addi32_typing_inv : forall t t1s t2s,
   t = term_addi32 ->
   typing t (Tf t1s t2s) ->
-  exists ts, t1s = ts ++ [t_i32; t_i32] ** t2s = ts ++ [t_i32].
+  {ts & t1s = ts ++ [t_i32; t_i32] /\ t2s = ts ++ [t_i32]}.
 Proof.
   intros t t1s t2s Hterm Htype.
-  subst t.
-  exists (removelast t2s); split.
+  subst t. exists (removelast t2s); split.
 Admitted.
 
 (* We beed a type checker for the remaining lemmas *)
@@ -97,47 +112,23 @@ Definition type_checker_seq (t1 t2: term) (tf1 tf2: function_type): function_typ
   end
 .
 
-(* assuming t well-typed, either:
- * * t2 consumes some of the output of t1 ('some' includes none or all)
- *   tf1=(Tf t1_in (ts ++ t2_in)) tf2=(Tf t2_in t2_out)
- *   (len t1_out >= t2_in)
- *   => so we need to consider weakened tf2:
- *   (Tf t1_in (ts ++ t2_in)) (Tf (ts ++ t2_in) (ts ++ t2_out))
- *   => the result is:
- *   Tf t1_in (ts ++ t2_out)
- *
- * * t2 consumes more than the output of t1,
- *   tf1=(Tf t1_in t1_out) tf2=(Tf (ts ++ t1_out) t2_out)
- *   (len t1_out <= t2_in)
- *   => so we need to consider weakened type of tf1:
- *   (Tf (ts ++ t1_in) (ts ++ t1_out)) (Tf (ts ++ t1_out) t2_out))
- *   => the result is:
- *   Tf (ts ++ t1_in) t2_out
- *)
-
-(*
-Tf qwer    efg
-Tf abcdefg xyz
-  -> weaken the first type as necessary
-Tf abcdqwer abcdefg
-Tf abcdefg  xyz
-  -> result:
-Tf abcdqwer xyz
- *)
-
 Fixpoint type_checker (t: term): function_type :=
   match t with
-  | term_i32 => Tf [] [t_i32]
-  | term_f32 => Tf [] [t_f32]
+  | term_const (val_i32 _) => Tf [] [t_i32]
+  | term_const (val_f32 _) => Tf [] [t_f32]
   | term_addi32 => Tf [t_i32; t_i32] [t_i32]
   | term_SEQ t1 t2 =>
       type_checker_seq t1 t2 (type_checker t1) (type_checker t2)
   end.
 
-Compute (type_checker term_i32).
-Compute (type_checker term_f32).
-Compute (type_checker (term_SEQ term_i32 term_f32)).
-Compute (type_checker (term_SEQ (term_SEQ term_i32 term_i32) term_addi32)).
+Let i_17 := term_const (val_i32 17).
+Let f_3_75 := term_const (val_f32 3.75).
+
+Compute (type_checker i_17).
+Compute (type_checker f_3_75).
+Compute (type_checker (term_SEQ i_17 f_3_75)).
+Compute (type_checker (term_SEQ (term_SEQ i_17 i_17) term_addi32)).
+Compute (type_checker (term_SEQ i_17 (term_SEQ i_17 term_addi32))).
 
 Axiom type_checker_implies_typing: forall t tf,
   type_checker t = tf ->
@@ -158,24 +149,76 @@ Lemma term_SEQ_typing_inv : forall t t1 t2 t1s t2s,
 Proof.
 Admitted.
 
-(* Note: the program given to the interpreter must take no input
- * XXX should change it to instead pass around the stack of values *)
-Definition interpret_one_step t tf_out (Htype : typing t (Tf [] tf_out)) : term.
+(* The value stack *)
+Definition stack := list value.
+
+Inductive stack_typing : stack -> list value_type -> Prop :=
+  | stack_typing_nil : stack_typing [] []
+  (* TODO stack type / naming *)
+  | stack_typing_cons : forall s st t vt,
+      stack_typing s st ->
+      value_typing t vt ->
+      stack_typing (t :: s) (vt :: st)
+.
+
+Lemma nil_stack_typing_inv : forall s, stack_typing s [] -> s = [].
+Proof. intros s Hstype. inversion Hstype. by reflexivity. Qed.
+
+Lemma cons_stack_typing_inv : forall s st t vt,
+  stack_typing (t :: s) (vt :: st) ->
+  stack_typing s st /\ value_typing t vt.
+Proof. intros s st t tt Hstype. inversion Hstype; auto. Qed.
+
+Lemma rcons_stack_typing_inv : forall s st t vt,
+  stack_typing (s ++ [t]) (st ++ [vt]) ->
+  stack_typing s st /\ value_typing t vt.
 Proof.
-  destruct t as [| | |t1 t2] eqn:teq.
-  (* term_i32 *)
-  - apply term_i32.
-  (* term_f32 *)
-  - apply term_f32.
-  (* term_addi32
-   * binop with no values available - violates Htype *)
-  - exfalso.
-    apply term_addi32_typing_inv in Htype as [ts [Hts _]] => //.
-    destruct ts; by inversion Hts.
-  (* term_SEQ *)
-  - apply (term_SEQ_typing_inv (term_SEQ t1 t2) _ _ _ _ eq_refl) in Htype
+  intros s st t tt Hstype.
+  induction s.
+Admitted.
+
+Lemma rcons_stack_typing_inv' : forall s st vt,
+  stack_typing s (st ++ [vt]) ->
+  {s' & {t & s = s' ++ [t] /\ stack_typing s' st /\ value_typing t vt}}.
+Proof. (* TODO *) Admitted.
+
+Lemma cat_stack_typing_inv : forall s st1 st2,
+  stack_typing s (st1 ++ st2) ->
+  {s1 & {s2 & s = s1 ++ s2 /\ stack_typing s1 st1 /\ stack_typing s2 st2}}.
+Proof. Admitted.
+
+(* Note: the stack given to the interpreter
+ * must contain the right type values *)
+Definition interpret_one_step
+  t tf_in tf_out s
+  (Htype : typing t (Tf tf_in tf_out)) (Hstype : stack_typing s tf_in)
+  : (term * stack).
+Proof.
+  destruct t as [| |t1 t2] eqn:teq.
+  - (* term_const *)
+    apply (t, s).
+  - (* term_addi32 *)
+    (* use Hstype to discover that the stack has at least two values on it *)
+    apply (term_addi32_typing_inv) in Htype as [ts [Hts1 Hts2]]; last by reflexivity.
+    subst tf_in.
+    assert (Hlist : ts ++ [t_i32; t_i32] = (ts ++ [t_i32]) ++ [t_i32]).
+    { rewrite <- app_assoc. by reflexivity. }
+    rewrite Hlist in Hstype.
+    apply (rcons_stack_typing_inv' s (ts ++ [t_i32])) in Hstype.
+    destruct Hstype as [s' [v1 [Hseq [Hstype Hvtype1]]]].
+    apply rcons_stack_typing_inv' in Hstype.
+    destruct Hstype as [s'' [v2 [Hseq1 [Hstype Hvtype2]]]].
+    subst s'.
+
+    (* now deduce t1 and t2 are both (term_const (val_i32 _)) *)
+    apply value_typing_inversion_i32 in Hvtype1 as [n1].
+    apply value_typing_inversion_i32 in Hvtype2 as [n2].
+    apply (term_const (val_i32 (n1 + n2)), s'').
+
+  - (* term_SEQ *)
+    apply (term_SEQ_typing_inv (term_SEQ t1 t2) _ _ _ _ eq_refl) in Htype
     as [ts [Htype1 Htype2]].
-    apply t. (* TODO just doing identity for now *)
+    apply (t, s). (* TODO just doing identity for now *)
 Defined.
 
 Recursive Extraction interpret_one_step.
